\subsection*{Obtaining the RegEx}
From the DFA in Fig:\ref{fig:comp_dfa}, we can obtain the following Equations
\begin{equation}
\label{eq:x1}
        X_1 = aX_2 \cup bX_4
        \end{equation}
\begin{equation}
\label{eq:x2}
        X_2 = aX_2 \cup bX_3
        \end{equation}
\begin{equation}
\label{eq:x3}
        X_3 = aX_2 \cup bX_4
        \end{equation}
\begin{equation}
\label{eq:x4}
        X_4 = (a\cup b)X_4 \cup \varepsilon
        \end{equation}
We need to find the regular expression for~$X_1$.

Applying Arden's lemma on equation \ref{eq:x4}, we obtain : 
\begin{equation}
    \label{eq:x4-2}
    X_4 = {(a \cup b)} ^*
\end{equation}
By Arden's lemma, eq:\ref{eq:x3} and the Distributive Law we can transform eq:\ref{eq:x2}:
\begin{equation}
    \label{eq:x2-2}
    \begin{split}
        &X_2 = aX_2 \cup baX_2 \cup bbX_4 \\
        &X_2 = {(a \cup ba)}^* bbX_4\\
    \end{split}
\end{equation}
Now substituting for $X_2$ and $X_4$ we obtain:
\begin{equation}
    X_1 = a{(a \cup ba)}^* bb{(a\cup b)}^* \; \cup \; b(a \cup b )^*
\end{equation}
